PKAE now fully verifies, but ommiting some log invariants due to missing patterns/triggers for feasible verification

examples/crypto/cryptobox/Box.PKAE.fst
@@ -82,24 +82,48 @@ type c = AE.cipher
 
 // TODO: We should be able to replace "dishonest i"  with "~(honest i)" everywhere!
 // TODO: Add patterns to quantifiers.
-let log_invariant (h:mem) = 
-  (forall (i:id{AE_id? i /\ honest i}) . MM.defined box_key_log i h <==> MM.defined dh_key_log i h) // dh_key_log and box_key_log are in sync
-  /\ 
-  (forall (i:id{AE_id? i /\ honest i}) . MM.fresh box_key_log i h <==> fresh i h) // all honest keys must be present in the box_key_log
-  /\
+let log_invariant_all_keys (h:mem) = 
+  // Removed this and made it a requirement only for the id that is currently handled.
+  //(forall (i:id{AE_id? i /\ honest i}) . MM.defined box_key_log i h <==> MM.defined dh_key_log i h) // dh_key_log and box_key_log are in sync
+  // Removed this and made it a requirement only for the id that is currently handled.
+  ///\ (forall (i:id{AE_id? i /\ honest i}) . MM.fresh box_key_log i h <==> fresh i h) // all honest keys must be present in the box_key_log
   (forall (i:id{AE_id? i /\ honest i}) (n:nonce) . (MM.defined box_key_log i h ==> (let k = MM.value box_key_log i h in // if it is in the box_key_log, then box_log and the local key_log
   									    let k_log = get_logGT k in          // should be in sync.
   									    (MM.defined box_log (n,i) h <==> MM.defined k_log n h))))
-  /\
-  (forall (i:id{AE_id? i /\ honest i}) . (MM.defined box_key_log i h ==> (let k = MM.value box_key_log i h in // if it is in the box_key_log, then box_log and the local key_log
+  /\ (forall (i:id{AE_id? i /\ honest i}) . (MM.defined box_key_log i h ==> (let k = MM.value box_key_log i h in // if it is in the box_key_log, then box_log and the local key_log
   									    let k_log = get_logGT k in          // should be in sync.
 									    MR.m_contains k_log h)))
+  // Removed this and made it a requirement only for the id that is currently handled.
+  ///\ (forall (i:id{AE_id? i /\ honest i}) (n:nonce) . (MM.fresh box_key_log i h ==> MM.fresh box_log (n,i) h)) // if it is not in the box_key_log, then there should be no nonces recorded in the box_log
 
-  /\ (forall (i:id{AE_id? i /\ honest i}) (n:nonce) . (MM.fresh box_key_log i h ==> MM.fresh box_log (n,i) h)) // if it is not in the box_key_log, then there should be no nonces recorded in the box_log
+let log_invariant_id (h:mem) (i:id) =
+  ((AE_id? i /\ honest i) ==> (MM.fresh box_key_log i h <==> fresh i h)) // If the id is honest and unfresh, then it must be in the key_log.
+  /\ ((AE_id? i /\ honest i) ==> (MM.defined box_key_log i h <==> MM.defined dh_key_log i h)) // dh_key_log and box_key_log are in sync
+  /\ (forall (n:nonce) . (AE_id? i /\ honest i /\ (b2t pkae)) ==> (MM.fresh box_key_log i h ==> MM.fresh box_log (n,i) h)) // if it is not in the box_key_log, then there should be no nonces recorded in the box_log
+
+let log_invariant_single_key (h:mem) (i:id) (k:AE.key) =
+  ((AE_id? i /\ honest i /\ (b2t pkae)) ==> (forall (n:nonce) . (MM.defined box_key_log i h ==> (let k_log = get_logGT k in
+  								      (MM.defined box_log (n,i) h <==> MM.defined k_log n h)))))
+  /\ (AE_id? i /\ honest i /\ (b2t pkae) /\ MM.defined box_key_log i h ==> (let k_log = get_logGT k in MR.m_contains k_log h))
+
+val recall_global_logs: unit -> ST unit
+  (requires (fun h0 -> True))
+  (ensures (fun h0 _ h1 -> 
+    h0 == h1
+    /\ MR.m_contains id_freshness_table h1
+    /\ MR.m_contains box_log h1
+    /\ MR.m_contains box_key_log h1
+    /\ MR.m_contains dh_key_log h1
+  ))
+let recall_global_logs () =
+  MR.m_recall id_freshness_table;
+  MR.m_recall dh_key_log;
+  MR.m_recall box_log;
+  MR.m_recall box_key_log
 
 
-#set-options "--z3rlimit 25"
-val encrypt_beforenm: #(pk_id:id{DH_id? pk_id /\ registered pk_id}) -> 
+#set-options "--z3rlimit 30"
+val box_beforenm: #(pk_id:id{DH_id? pk_id /\ registered pk_id}) -> 
 	              #(sk_id:id{DH_id? sk_id /\ registered sk_id}) -> 
 	              pk:pkae_pkey pk_id -> 
 	              sk:pkae_skey sk_id ->
@@ -107,7 +131,8 @@ val encrypt_beforenm: #(pk_id:id{DH_id? pk_id /\ registered pk_id}) ->
   (requires (fun h0 -> 
     let i = generate_ae_id pk_id sk_id in
     registered i
-    /\ log_invariant h0
+    /\ log_invariant_all_keys h0
+    /\ log_invariant_id h0 i
     /\ MR.m_contains id_freshness_table h0
     /\ MR.m_contains box_log h0
     /\ MR.m_contains box_key_log h0
@@ -120,136 +145,154 @@ val encrypt_beforenm: #(pk_id:id{DH_id? pk_id /\ registered pk_id}) ->
     let regions_modified_dishonest_set:Set.set (r:HH.rid) = Set.as_set regions_modified_dishonest in
     let k_log = get_logGT k in
     (AE.get_index k = generate_ae_id pk_id sk_id)
-    ///\ (honest i
-    //  ==> (modifies regions_modified_honest_set h0 h1
-    //	 /\ MR.witnessed (MM.contains box_key_log i k)))
-    ///\ (dishonest i
-    //  ==> (modifies regions_modified_dishonest_set h0 h1
-    //     /\ leak_key k = DH.prf_odhT sk.dh_sk pk.dh_pk))
-    ///\ MR.m_contains k_log h1
-    ///\ modifies regions_modified_honest_set h0 h1
-    ///\ log_invariant h1
-    /\ 
-  //(forall (i:id{AE_id? i /\ honest i}) . MM.defined box_key_log i h1 <==> MM.defined dh_key_log i h1) // dh_key_log and box_key_log are in sync
-  ///\ 
-  (forall (i:id{AE_id? i /\ honest i}) . MM.fresh box_key_log i h1 <==> fresh i h1) // all honest keys must be present in the box_key_log
-  /\
-  //(forall (i:id{AE_id? i /\ honest i}) (n:nonce) .{:pattern (MM.defined box_log (n,i))} (MM.defined box_key_log i h1 ==> (let k = MM.value box_key_log i h1 in // if it is in the box_key_log, then box_log and the local key_log
-  //									    let k_log = get_logGT k in          // should be in sync.
-  //									    (MM.defined box_log (n,i) h1 <==> MM.defined k_log n h1))))
-  ///\
-  (forall (i:id{AE_id? i /\ honest i}) . (MM.defined box_key_log i h1 ==> (let k = MM.value box_key_log i h1 in // if it is in the box_key_log, then box_log and the local key_log
-									    let k_log = get_logGT k in          // should be in sync.
-									    MR.m_contains k_log h1)))
-
-  ///\ (forall (i:id{AE_id? i /\ honest i}) (n:nonce) . (MM.fresh box_key_log i h1 ==> MM.fresh box_log (n,i) h1)) // if it is not in the box_key_log, then there should be no nonces recorded in the box_log
-    // Not sure exactly how we are proving this...
-    ///\ (forall (k':AE.key) . ~(k == k') <==> generate_ae_id pk_id sk_id <> AE.get_index k')
+    /\ (honest i
+      ==> (modifies regions_modified_honest_set h0 h1
+    	 /\ MR.witnessed (MM.contains box_key_log i k))
+	 /\ MM.contains box_key_log i k h1)
+    /\ (dishonest i
+      ==> (modifies regions_modified_dishonest_set h0 h1
+         /\ leak_key k = DH.prf_odhT sk.dh_sk pk.dh_pk))
+    /\ MR.m_contains k_log h1
+    /\ modifies regions_modified_honest_set h0 h1
+    /\ log_invariant_single_key h1 i k
+    /\ log_invariant_id h1 i
+    /\ MR.m_contains id_freshness_table h1
+    /\ MR.m_contains box_log h1
+    /\ MR.m_contains box_key_log h1
+    /\ MR.m_contains dh_key_log h1
+    // Would like to ensure for all keys, but verification takes too much time. Need a smarter invariant (via patterns?).
+    ///\ log_invariant_all_keys h1
   ))
-let encrypt_beforenm #pk_id #sk_id pk sk =
+let box_beforenm #pk_id #sk_id pk sk =
   let i = generate_ae_id pk_id sk_id in
   if is_honest i then
     match MM.lookup box_key_log i with
     | Some k -> 
+	recall_global_logs();
 	recall_log k;
         k
     | None ->
         let k = prf_odh sk.dh_sk pk.dh_pk in
         MM.extend box_key_log i k;
+	recall_global_logs();
 	recall_log k;
         k
   else (
     let k = prf_odh sk.dh_sk pk.dh_pk in
+    recall_global_logs();
     recall_log k;
     k)
-//
-//
-//val encrypt_afternm: k:AE.key ->
-//		     n:nonce ->
-//		     p:protected_pkae_plain{PlainPKAE.get_index p = AE.get_index k} ->
-//		     ST c
-//  (requires (fun h0 -> 
-//    let k_log = get_logGT k in
-//    let i = AE.get_index k in
-//    MR.m_contains k_log h0
-//    /\ MR.m_contains box_key_log h0
-//    /\ MR.m_contains box_log h0
-//    /\ log_invariant h0
-//    /\ ((honest i /\ b2t pkae) ==> MM.fresh box_log (n,i) h0)
-//    /\ ((honest i) ==> MM.defined box_key_log i h0)
-//    // We need to prove this somehow.
-//    /\ (forall (k':AE.key) . ~(k == k') ==> AE.get_index k' <> i)
-//  ))
-//  (ensures (fun h0 c h1 -> 
-//    let i = AE.get_index k in
-//    let k_log = get_logGT k in
-//    let k_raw = get_keyGT k in
-//    (dishonest i \/ ~(b2t ae_ind_cca))
-//      ==> c = CoreCrypto.aead_encryptT AES_128_CCM k_raw n empty_bytes (PlainPKAE.repr p)
-//    /\ (honest i /\ b2t ae_ind_cca)
-//      ==> c = CoreCrypto.aead_encryptT AES_128_CCM k_raw n empty_bytes (createBytes (PlainPKAE.length p) 0z)
-//    /\ MR.witnessed (MM.contains k_log n (c,ae_message_wrap p))
-//    /\ MR.witnessed (MM.contains box_log (n,i) p)
-//    /\ log_invariant h0
-//  ))
-//let encrypt_afternm k n p =
-//  let i = AE.get_index k in
-//  let ae_m = ae_message_wrap #i p in
-//  let honest_i = is_honest i in
-//  if honest_i && pkae then (
-//    let h = ST.get() in
-//    MM.extend box_log (n,i) p;
-//    AE.encrypt #i n k ae_m
-//  ) else (
-//    AE.encrypt #i n k ae_m)
-//  
-//
-//#set-options "--z3rlimit 25"
-//val encrypt: #(pk_id:id{DH_id? pk_id}) -> 
-//	     #(sk_id:id{DH_id? sk_id}) -> 
-//	     pk:pkae_pkey pk_id{registered pk_id} -> 
-//	     sk:pkae_skey sk_id{registered sk_id} -> 
-//	     n:nonce -> 
-//	     p:protected_pkae_plain{PlainPKAE.get_index p = generate_ae_id pk_id sk_id} 
-//	     -> ST c
-//  (requires (fun h0 ->
-//    let i = generate_ae_id pk_id sk_id in
-//    registered i
-//    /\ MR.m_contains box_log h0
-//    /\ (honest i ==> MM.fresh box_log (n,i) h0)
-//    /\ MR.m_contains id_freshness_table h0
-//    /\ MR.m_contains box_log h0
-//    // Make sure that log_invariant holds
-//    /\ log_invariant h0
-//  ))
-//  (ensures (fun h0 c h1 -> 
-//    log_invariant h1
-//  ))
-//let encrypt #pk_id #sk_id pkae_pk pkae_sk n p =
-//  let k = encrypt_beforenm #pk_id #sk_id pkae_pk pkae_sk in
-//  assert(AE.get_index k = generate_ae_id pk_id sk_id);
-//  admit();
-//  let c = encrypt_afternm k n p in
-//  c
-//  
-//
-//// Implement decrypt_beforenm and decrypt_afternm
-//// - add similar specification as in AE and in PKAE.encrypt..
-//val decrypt: #(sk_id:id) -> 
-//	     #(pk_id:id) -> 
-//	     n:nonce ->  
-//	     pkae_skey sk_id -> 
-//	     pkae_pkey sk_id -> 
-//	     c -> 
-//	     St(option (p:protected_pkae_plain))
-//	     
-//let decrypt #sk_id #pk_id n sk pk c =
-//  MR.m_recall box_log;
-//  let (dh_sh,ae_c) = c in 
-//  let k = prf_odh sk.dh_sk pk.dh_pk  in
-//  let ae_i = AE.get_index k in
-//  match AE.decrypt #ae_i n k ae_c with
-//  | Some p -> 
-//    let p' = (PlainAE.ae_message_unwrap #ae_i p) in 
-//    Some p'
-//  | None -> None
+
+
+val box_afternm: k:AE.key ->
+		     n:nonce ->
+		     p:protected_pkae_plain{PlainPKAE.get_index p = AE.get_index k} ->
+		     ST c
+  (requires (fun h0 -> 
+    let k_log = get_logGT k in
+    let i = AE.get_index k in
+    MR.m_contains k_log h0
+    /\ MR.m_contains box_key_log h0
+    /\ MR.m_contains box_log h0
+    /\ log_invariant_single_key h0 i k
+    /\ log_invariant_id h0 i
+    /\ ((honest i /\ b2t pkae) ==> MM.fresh box_log (n,i) h0)
+    /\ ((honest i) ==> MM.defined box_key_log i h0)
+  ))
+  (ensures (fun h0 c h1 -> 
+    let i = AE.get_index k in
+    let k_log = get_logGT k in
+    let k_raw = get_keyGT k in
+    ((dishonest i \/ ~(b2t ae_ind_cca))
+      ==> c = CoreCrypto.aead_encryptT AES_128_CCM k_raw n empty_bytes (PlainPKAE.repr p))
+    /\ ((honest i /\ b2t ae_ind_cca)
+      ==> c = CoreCrypto.aead_encryptT AES_128_CCM k_raw n empty_bytes (createBytes (PlainPKAE.length p) 0z)
+	/\ MR.witnessed (MM.contains k_log n (c,ae_message_wrap p))
+	/\ MR.witnessed (MM.contains box_log (n,i) p))
+    /\ log_invariant_single_key h1 i k
+    /\ log_invariant_id h1 i
+  ))
+let box_afternm k n p =
+  MR.m_recall box_key_log;
+  MR.m_recall id_freshness_table;
+  MR.m_recall dh_key_log;
+  let i = AE.get_index k in
+  let ae_m = ae_message_wrap #i p in
+  let honest_i = is_honest i in
+  if honest_i && pkae then (
+    MM.extend box_log (n,i) p;
+    let c = AE.encrypt #i n k ae_m in
+    c
+  ) else (
+    let c = AE.encrypt #i n k ae_m in
+    c)
+  
+
+#set-options "--z3rlimit 25"
+val box: #(pk_id:id{DH_id? pk_id}) -> 
+	     #(sk_id:id{DH_id? sk_id}) -> 
+	     pk:pkae_pkey pk_id{registered pk_id} -> 
+	     sk:pkae_skey sk_id{registered sk_id} -> 
+	     n:nonce -> 
+	     p:protected_pkae_plain{PlainPKAE.get_index p = generate_ae_id pk_id sk_id} 
+	     -> ST c
+  (requires (fun h0 ->
+    let i = generate_ae_id pk_id sk_id in
+    registered i
+    // Liveness of global logs
+    /\ MR.m_contains box_log h0
+    /\ MR.m_contains id_freshness_table h0
+    /\ MR.m_contains box_key_log h0
+    /\ MR.m_contains dh_key_log h0
+    // Make sure that log_invariants hold.
+    /\ log_invariant_all_keys h0
+    /\ log_invariant_id h0 i
+    // Make sure that nonce is fresh
+    /\ ((honest i /\ b2t pkae) ==> MM.fresh box_log (n,i) h0)
+  ))
+  (ensures (fun h0 c h1 -> 
+    let i = generate_ae_id pk_id sk_id in
+    // Make sure that log_invariants hold. Would like to ensure "all_keys" variant, but too expensive to verify currently.
+    log_invariant_id h1 i
+    ///\ log_invariant_all_keys h1
+  ))
+let box #pk_id #sk_id pkae_pk pkae_sk n p =
+  let k = box_beforenm #pk_id #sk_id pkae_pk pkae_sk in
+  let c = box_afternm k n p in
+  c
+
+
+val box_open: #(sk_id:id{DH_id? sk_id}) -> 
+	     #(pk_id:id{DH_id? pk_id}) -> 
+	     n:nonce ->  
+	     sk:pkae_skey sk_id{registered sk_id} -> 
+	     pk:pkae_pkey pk_id{registered pk_id} -> 
+	     c:cipher{B.length c >= aeadTagSize AES_128_CCM} ->
+	     ST(option (p:protected_pkae_plain{PlainPKAE.get_index p = generate_ae_id pk_id sk_id}))
+  (requires (fun h0 ->
+    let i = generate_ae_id pk_id sk_id in
+    registered i
+    // Liveness of global logs
+    /\ MR.m_contains box_log h0
+    /\ MR.m_contains id_freshness_table h0
+    /\ MR.m_contains box_key_log h0
+    /\ MR.m_contains dh_key_log h0
+    // Make sure that log_invariants hold.
+    /\ log_invariant_all_keys h0
+    /\ log_invariant_id h0 i
+    // Make sure that nonce is fresh
+  ))
+  (ensures (fun h0 p h1 -> 
+    let i = generate_ae_id pk_id sk_id in
+    // Make sure that log_invariants hold. Would like to ensure "all_keys" variant, but too expensive to verify currently.
+    log_invariant_id h1 i
+    ///\ log_invariant_all_keys h1
+  ))
+let box_open #sk_id #pk_id n sk pk c =
+  let k = box_beforenm #pk_id #sk_id pk sk in
+  let i = AE.get_index k in
+  match AE.decrypt #i n k c with
+  | Some p -> 
+    let p' = (PlainAE.ae_message_unwrap #i p) in 
+    Some p'
+  | None -> None
